Lynx/Modules/Maps.lean
@@ -3,7 +3,7 @@ import Lynx.Tactic
 namespace Lynx.Modules.Maps
 open Term.Map
 
-#lynx_pure def new_0 : Result := .ok Term.empty_map
+#lynx_pure def new_0 : Result := .ok Term.emptyMap
 
 #lynx_pure @[lynx_opaque] def get_2 (key input : Term) : Result :=
   match input with
@@ -36,6 +36,6 @@ open Term.Map
     merge_2 (.map a) (.map b) = .ok (.map (merge a b)) := rfl
 
 @[simp] theorem merge_empty_right (entries : Entries) :
-    merge_2 (.map entries) Term.empty_map = .ok (.map entries) := rfl
+    merge_2 (.map entries) Term.emptyMap = .ok (.map entries) := rfl
 
 end Lynx.Modules.Maps
